#algebra 
The substitution method is a technique for solving systems of linear equations. This method involves solving one of the equations for one variable in terms of the other(s) and then substituting this expression into the other equation(s). This method is particularly useful when one of the equations is easily solvable for one of the variables. Here’s how you can use the substitution method step-by-step:

### Steps to Solve Using the Substitution Method

1. **Solve one of the equations for one of its variables.**
   - Look for the equation and variable that is easiest to solve for. It doesn't matter which one you choose, but generally, you want to minimize the amount of work you have to do.

2. **Substitute the expression found in step 1 into the other equation.**
   - Replace the variable you solved for in step 1 with the expression you found throughout the other equation(s). This gives you an equation with one variable.

3. **Solve the resulting equation from step 2.**
   - This step should give you the value of one of the variables.

4. **Substitute the value found in step 3 back into any equation involving both variables to solve for the other variable.**
   - You can use the original equation you modified in step 1 or any other equation in the system that includes both variables.

5. **Check your solution in both original equations.**
   - Substituting your solutions back into the original equations should satisfy both equations. If it doesn’t, recheck your work.

### Example

Let's solve the system of equations using the substitution method:

1. $x + 2y = 5$
2. $3x - y = 4$

**Step 1:** Solve the first equation for $x$:

$x = 5 - 2y$

**Step 2:** Substitute $x = 5 - 2y$ into the second equation:

$3(5 - 2y) - y = 4$

**Step 3:** Solve for $y$:

$15 - 6y - y = 4$
$-7y = -11$
$y = \frac{11}{7}$

**Step 4:** Substitute $y = \frac{11}{7}$ back into $x = 5 - 2y$:

$x = 5 - 2\left(\frac{11}{7}\right)$
$x = \frac{35}{7} - \frac{22}{7}$
$x = \frac{13}{7}$

**Step 5:** Check the solution $(x, y) = \left(\frac{13}{7}, \frac{11}{7}\right)$ in both original equations:

For $x + 2y = 5$:
$\frac{13}{7} + 2\left(\frac{11}{7}\right) = \frac{13}{7} + \frac{22}{7} = \frac{35}{7} = 5$

For $3x - y = 4$:
$3\left(\frac{13}{7}\right) - \frac{11}{7} = \frac{39}{7} - \frac{11}{7} = \frac{28}{7} = 4$

Both equations are satisfied, so the solution is correct: $(x, y) = \left(\frac{13}{7}, \frac{11}{7}\right)$.

